lambda2Gmu/CanonicalForms.v
@@ -5,8 +5,8 @@ Require Import TLC.LibEnv.
 Require Import TLC.LibLN.
 
   (* Ht : {Σ, empty}⊢ trm_constructor Tparams Name e1 ∈ T1 ** T2 *)
-Lemma CanonicalConstructorType : forall Σ E Tparams Name Ctor e1 T,
-    {Σ, E} ⊢ trm_constructor Tparams (Name, Ctor) e1 ∈ T ->
+Lemma CanonicalConstructorType : forall Σ Δ E Tparams Name Ctor e1 T,
+    {Σ, Δ, E} ⊢ trm_constructor Tparams (Name, Ctor) e1 ∈ T ->
     (* TODO can we make Typs more specific? *)
     exists Typs, T = typ_gadt Typs Name.
   introv Htyp.
@@ -16,8 +16,8 @@ Lemma CanonicalConstructorType : forall Σ E Tparams Name Ctor e1 T,
   f_equal.
 Qed.
 
-Lemma CanonicalConstructorTypeGen : forall Σ E Tparams Ctor e1 T,
-    {Σ, E} ⊢ trm_constructor Tparams Ctor e1 ∈ T ->
+Lemma CanonicalConstructorTypeGen : forall Σ Δ E Tparams Ctor e1 T,
+    {Σ, Δ, E} ⊢ trm_constructor Tparams Ctor e1 ∈ T ->
     (* TODO can we make Typs more specific? *)
     exists Typs Name, T = typ_gadt Typs Name.
   intros.
@@ -31,57 +31,57 @@ Hint Resolve CanonicalConstructorTypeGen.
 
 Ltac contradictory_constructor_type :=
   lazymatch goal with
-  | H: {?S, ?E} ⊢ trm_constructor ?Ts ?C ?e ∈ ?T |- _ =>
+  | H: {?S, ?D, ?E} ⊢ trm_constructor ?Ts ?C ?e ∈ ?T |- _ =>
     apply CanonicalConstructorTypeGen in H;
     let Hcontradict := fresh "contradict" in
     destruct H as [? [? Hcontradict]];
     inversion Hcontradict
   end.
 
-Lemma CanonicalFormTuple : forall Σ e T1 T2,
+Lemma CanonicalFormTuple : forall Σ Δ E e T1 T2,
     value e ->
-    {Σ, empty} ⊢ e ∈ T1 ** T2 ->
+    {Σ, Δ, E} ⊢ e ∈ T1 ** T2 ->
     exists v1 v2, e = trm_tuple v1 v2.
   introv Hv Ht.
   inversion Hv; inversion Ht; subst; eauto; try congruence.
   contradictory_constructor_type.
 Qed.
 
-Lemma CanonicalFormAbs : forall Σ e T1 T2,
+Lemma CanonicalFormAbs : forall Σ Δ E e T1 T2,
     value e ->
-    {Σ, empty} ⊢ e ∈ T1 ==> T2 ->
+    {Σ, Δ, E} ⊢ e ∈ T1 ==> T2 ->
     exists v1, e = trm_abs T1 v1.
   introv Hv Ht.
   inversion Hv; inversion Ht; subst; eauto; try congruence.
   contradictory_constructor_type.
 Qed.
 
-Lemma CanonicalFormTAbs : forall Σ e T,
+Lemma CanonicalFormTAbs : forall Σ Δ E e T,
     value e ->
-    {Σ, empty} ⊢ e ∈ typ_all T ->
+    {Σ, Δ, E} ⊢ e ∈ typ_all T ->
     exists v1, e = trm_tabs v1.
   introv Hv Ht.
   inversion Hv; inversion Ht; subst; eauto; try congruence.
   contradictory_constructor_type.
 Qed.
 
-Lemma CanonicalFormUnit : forall Σ e,
+Lemma CanonicalFormUnit : forall Σ Δ E e,
     value e ->
-    {Σ, empty} ⊢ e ∈ typ_unit ->
+    {Σ, Δ, E} ⊢ e ∈ typ_unit ->
     e = trm_unit.
   introv Hv Ht.
   inversion Hv; inversion Ht; subst; eauto; try congruence.
   contradictory_constructor_type.
 Qed.
 
-Lemma CanonicalFormGadt : forall Σ e Ts N,
+Lemma CanonicalFormGadt : forall Σ Δ E e Ts N,
     value e ->
-    {Σ, empty} ⊢ e ∈ typ_gadt Ts N ->
+    {Σ, Δ, E} ⊢ e ∈ typ_gadt Ts N ->
     exists Ts' C v, e = trm_constructor Ts' (N, C) v. (* todo may want to relate Ts' to Ts *)
   introv Hv Ht.
   inversion Hv; inversion Ht; subst; eauto; try congruence.
   rewrite rewrite_open_tt_many_gadt in H8.
   inversions H8.
-  inversions H11.
+  inversions H12.
   repeat eexists.
 Qed.
