lambda2Gmu/Infrastructure.v
@@ -1089,48 +1089,48 @@ Fixpoint subst_tb_many (As : list var) (Us : list typ) (b : bind) : bind :=
   | _ => b
   end.
 
-Lemma adding_free_is_ok : forall A E F,
-    ok (E & F) ->
-    A # E ->
-    A # F ->
-    ok (E & (withtyp A) & F)%env.
-  induction F using env_ind; introv Hok HE HF.
-  - rewrite concat_empty_r.
-    constructor*.
-  - rewrite concat_assoc.
-    rewrite concat_assoc in Hok.
-    apply ok_push_inv in Hok.
-    econstructor.
-    + apply* IHF.
-    + simpl_dom.
-      rewrite notin_union.
-      rewrite notin_union.
-      split*.
-Qed.
+(* Lemma adding_free_is_ok : forall A E F, *)
+(*     ok (E & F) -> *)
+(*     A # E -> *)
+(*     A # F -> *)
+(*     ok (E & (withtyp A) & F)%env. *)
+(*   induction F using env_ind; introv Hok HE HF. *)
+(*   - rewrite concat_empty_r. *)
+(*     constructor*. *)
+(*   - rewrite concat_assoc. *)
+(*     rewrite concat_assoc in Hok. *)
+(*     apply ok_push_inv in Hok. *)
+(*     econstructor. *)
+(*     + apply* IHF. *)
+(*     + simpl_dom. *)
+(*       rewrite notin_union. *)
+(*       rewrite notin_union. *)
+(*       split*. *)
+(* Qed. *)
 
-Lemma adding_free_is_ok_many : forall As E F,
-    ok (E & F) ->
-    DistinctList As ->
-    (forall A, List.In A As -> A \notin dom E) ->
-    (forall A, List.In A As -> A \notin dom F) ->
-    ok (add_types E As & F).
-  induction As as [| Ah Ats]; introv Hok HD HE HF.
-  - cbn. eauto.
-  - cbn.
-    rewrite <- concat_assoc.
-    apply IHAts; eauto with listin.
-    + rewrite concat_assoc.
-      apply adding_free_is_ok; eauto with listin.
-    + inversion* HD.
-    + introv Hin.
-      simpl_dom.
-      rewrite notin_union.
-      split.
-      * apply* notin_singleton.
-        inversions HD.
-        intro; subst. contradiction.
-      * eauto with listin.
-Qed.
+(* Lemma adding_free_is_ok_many : forall As E F, *)
+(*     ok (E & F) -> *)
+(*     DistinctList As -> *)
+(*     (forall A, List.In A As -> A \notin dom E) -> *)
+(*     (forall A, List.In A As -> A \notin dom F) -> *)
+(*     ok (add_types E As & F). *)
+(*   induction As as [| Ah Ats]; introv Hok HD HE HF. *)
+(*   - cbn. eauto. *)
+(*   - cbn. *)
+(*     rewrite <- concat_assoc. *)
+(*     apply IHAts; eauto with listin. *)
+(*     + rewrite concat_assoc. *)
+(*       apply adding_free_is_ok; eauto with listin. *)
+(*     + inversion* HD. *)
+(*     + introv Hin. *)
+(*       simpl_dom. *)
+(*       rewrite notin_union. *)
+(*       split. *)
+(*       * apply* notin_singleton. *)
+(*         inversions HD. *)
+(*         intro; subst. contradiction. *)
+(*       * eauto with listin. *)
+(* Qed. *)
 
 Lemma fv_typs_notin : forall Ts T X,
     List.In T Ts ->
@@ -1286,29 +1286,29 @@ Lemma fold_empty : forall Ts,
   eauto with listin.
 Qed.
 
-Lemma add_types_map_subst_tb : forall As Z P,
-    map (subst_tb Z P) (add_types empty As)
-    =
-    add_types empty As.
-  induction As as [| Ah Ats]; introv.
-  - cbn. autorewrite with rew_env_map. trivial.
-  - cbn. autorewrite with rew_env_map. cbn. rewrite IHAts. trivial.
-Qed.
+(* Lemma add_types_map_subst_tb : forall As Z P, *)
+(*     map (subst_tb Z P) (add_types empty As) *)
+(*     = *)
+(*     add_types empty As. *)
+(*   induction As as [| Ah Ats]; introv. *)
+(*   - cbn. autorewrite with rew_env_map. trivial. *)
+(*   - cbn. autorewrite with rew_env_map. cbn. rewrite IHAts. trivial. *)
+(* Qed. *)
 
-Lemma add_types_through_map : forall Z P E F As,
-    map (subst_tb Z P) (add_types E As & F)
-    =
-    add_types (map (subst_tb Z P) E) As & (map (subst_tb Z P) F).
-  intros.
-  autorewrite with rew_env_map.
-  f_equal.
-  rewrite <- (concat_empty_r E).
-  rewrite add_types_assoc.
-  autorewrite with rew_env_map.
-  rewrite add_types_assoc.
-  f_equal.
-  apply add_types_map_subst_tb.
-Qed.
+(* Lemma add_types_through_map : forall Z P E F As, *)
+(*     map (subst_tb Z P) (add_types E As & F) *)
+(*     = *)
+(*     add_types (map (subst_tb Z P) E) As & (map (subst_tb Z P) F). *)
+(*   intros. *)
+(*   autorewrite with rew_env_map. *)
+(*   f_equal. *)
+(*   rewrite <- (concat_empty_r E). *)
+(*   rewrite add_types_assoc. *)
+(*   autorewrite with rew_env_map. *)
+(*   rewrite add_types_assoc. *)
+(*   f_equal. *)
+(*   apply add_types_map_subst_tb. *)
+(* Qed. *)
 
 Lemma fv_smaller_many : forall As T,
     fv_typ (open_tt_many_var As T) \c (fv_typ T \u from_list As).
